code/experimental/poly1305/Hacl.Impl.Poly1305.fsti
@@ -16,56 +16,57 @@ module F32xN = Hacl.Impl.Poly1305.Field32xN
 #reset-options "--z3rlimit 50"
 
 inline_for_extraction
+type poly1305_ctx (s:field_spec) = lbuffer (limb s) (nlimb s +. precomplen s)
+
+noextract
+val as_get_acc: #s:field_spec -> h:mem -> ctx:poly1305_ctx s -> GTot (S.elem (width s))
+noextract
+val as_get_r: #s:field_spec -> h:mem -> ctx:poly1305_ctx s -> GTot (S.elem (width s))
+noextract
+val state_inv_t: #s:field_spec -> h:mem -> ctx:poly1305_ctx s -> Type0
+
+inline_for_extraction
 val poly1305_init:
     #s:field_spec
+  -> ctx:poly1305_ctx s
   -> key:lbuffer uint8 32ul
-  -> pre:precomp_r s
-  -> acc:felem s
   -> Stack unit
     (requires fun h ->
-      live h pre /\ live h acc /\  live h key /\
-      disjoint pre key /\ disjoint acc key /\
-      disjoint pre acc)
+      live h ctx /\ live h key /\ disjoint ctx key)
     (ensures  fun h0 _ h1 ->
-      modifies (loc acc |+| loc pre) h0 h1 /\
-      F32xN.load_precompute_r_post #(width s) h1 pre /\
-      felem_fits h1 acc (0, 0, 0, 0, 0) /\
-      (feval h1 acc, feval h1 (gsub pre 0ul 5ul)) == S.poly1305_init (as_seq h0 key))
+      modifies (loc ctx) h0 h1 /\
+      state_inv_t #s h1 ctx /\
+      (as_get_acc h1 ctx, as_get_r h1 ctx) == S.poly1305_init (as_seq h0 key))
 
 inline_for_extraction
 val poly1305_update:
     #s:field_spec
+  -> ctx:poly1305_ctx s
   -> len:size_t
   -> text:lbuffer uint8 len
-  -> pre:precomp_r s
-  -> acc:felem s
   -> Stack unit
     (requires fun h ->
-      live h text /\ live h acc /\ live h pre /\
-      disjoint acc text /\ disjoint acc pre /\
-      F32xN.acc_inv_t #(width s) (F32xN.as_tup5 h acc) /\
-      F32xN.load_precompute_r_post #(width s) h pre)
+      live h text /\ live h ctx /\ disjoint ctx text /\
+      state_inv_t #s h ctx)
     (ensures  fun h0 _ h1 ->
-      modifies (loc acc) h0 h1 /\
-      F32xN.acc_inv_t #(width s) (F32xN.as_tup5 h1 acc) /\
-      feval h1 acc ==
-      S.poly #(width s) (as_seq h0 text) (feval h0 acc) (feval h0 (gsub pre 0ul 5ul)))
+      modifies (loc ctx) h0 h1 /\
+      state_inv_t #s h1 ctx /\
+      as_get_acc h1 ctx == S.poly #(width s) (as_seq h0 text) (as_get_acc h0 ctx) (as_get_r h0 ctx))
 
-inline_for_extraction noextract
+inline_for_extraction
 val poly1305_finish:
     #s:field_spec
-  -> key:lbuffer uint8 32ul
-  -> acc:felem s
   -> tag:lbuffer uint8 16ul
+  -> key:lbuffer uint8 32ul
+  -> ctx:poly1305_ctx s
   -> Stack unit
     (requires fun h ->
-      live h acc /\ live h tag /\ live h key /\
-      disjoint acc tag /\ disjoint key tag /\
-      disjoint acc key /\
-      F32xN.acc_inv_t #(width s) (F32xN.as_tup5 h acc))
+      live h tag /\ live h key /\ live h ctx /\
+      disjoint tag key /\ disjoint tag ctx /\ disjoint key ctx /\
+      state_inv_t #s h ctx)
     (ensures  fun h0 _ h1 ->
-      modifies (loc tag |+| loc acc) h0 h1 /\
-      as_seq h1 tag == S.finish #(width s) (as_seq h0 key) (feval h0 acc))
+      modifies (loc tag |+| loc ctx) h0 h1 /\
+      as_seq h1 tag == S.finish #(width s) (as_seq h0 key) (as_get_acc h0 ctx))
 
 inline_for_extraction
 val poly1305_mac:
